Checkpoint.

src/coq/Handlers/MemoryModel.v
@@ -2014,6 +2014,7 @@ Module Type MemoryExecMonad (LP : LLVMParams) (MP : MemoryParams LP) (MMSP : Mem
         `{MPROV : MonadProvenance Provenance M} `{MSID : MonadStoreId M} `{MMS: MonadMemState MemState M}
         `{MERR : RAISE_ERROR M} `{MUB : RAISE_UB M} `{MOOM :RAISE_OOM M}
         `{RunERR : RAISE_ERROR RunM} `{RunUB : RAISE_UB RunM} `{RunOOM :RAISE_OOM RunM}
+        `{EQM : Eq1 M} `{MLAWS : @MonadLawsE M EQM MM}
     : Type
     :=
     { MemMonad_eq1_runm :> Eq1 RunM;
@@ -2122,9 +2123,9 @@ Module Type MemoryExecMonad (LP : LLVMParams) (MP : MemoryParams LP) (MMSP : Mem
     (*** Correctness *)
     Definition exec_correct {MemM Eff ExtraState} `{MM: MemMonad ExtraState MemM (itree Eff)} {X} (exec : MemM X) (spec : MemPropT MemState X) : Prop :=
       forall ms st,
-        (@MemMonad_valid_state ExtraState MemM (itree Eff) _ _ _ _ _ _ _ _ _ _ _ _ ms st) ->
+        (@MemMonad_valid_state ExtraState MemM (itree Eff) _ _ _ _ _ _ _ _ _ _ _ _ _ _ ms st) ->
         let t := MemMonad_run exec ms st in
-        let eqi := (@eq1 _ (@MemMonad_eq1_runm _ _ _ _ _ _ _ _ _ _ _ _ _ _ MM)) in
+        let eqi := (@eq1 _ (@MemMonad_eq1_runm _ _ _ _ _ _ _ _ _ _ _ _ _ _ _ _ MM)) in
         (* UB *)
         (exists msg_spec,
             spec ms (raise_ub msg_spec)) \/
@@ -2140,7 +2141,7 @@ Module Type MemoryExecMonad (LP : LLVMParams) (MP : MemoryParams LP) (MMSP : Mem
           (exists st' ms' x,
               eqi _ t (ret (st', (ms', x))) /\
                 spec ms (ret (ms', x)) /\
-                (@MemMonad_valid_state ExtraState MemM (itree Eff) _ _ _ _ _ _ _ _ _ _ _ _ ms' st')).
+                (@MemMonad_valid_state ExtraState MemM (itree Eff) _ _ _ _ _ _ _ _ _ _ _ _ _ _ ms' st')).
 
     Definition exec_correct_memory {MemM Eff ExtraState} `{MM: MemMonad ExtraState MemM (itree Eff)} {X} (exec : MemM X) (spec : MemPropT memory_stack X) : Prop :=
       exec_correct exec (lift_memory_MemPropT spec).
@@ -2183,7 +2184,7 @@ Module Type MemoryExecMonad (LP : LLVMParams) (MP : MemoryParams LP) (MMSP : Mem
             exec_correct (k_exec a) (k_spec a)) ->
         exec_correct (a <- m_exec;; k_exec a) (a <- m_spec;; k_spec a).
     Proof.
-      intros MemM Eff ExtraState MM MRun MPROV MSID MMS MERR MUB MOOM RunERR RunUB RunOOM MEMM A B m_exec k_exec m_spec k_spec M_CORRECT K_CORRECT.
+      intros MemM Eff ExtraState MM MRun MPROV MSID MMS MERR MUB MOOM RunERR RunUB RunOOM EQM MLAWS MEMM A B m_exec k_exec m_spec k_spec M_CORRECT K_CORRECT.
 
       unfold exec_correct in *.
       intros ms st VALID.
@@ -2284,7 +2285,7 @@ Module Type MemoryExecMonad (LP : LLVMParams) (MP : MemoryParams LP) (MMSP : Mem
         (forall a, exec_correct (k_exec a) (k_spec a)) ->
         exec_correct (a <- m_exec;; k_exec a) (a <- m_spec;; k_spec a).
     Proof.
-      intros MemM Eff ExtraState MM MRun MPROV MSID MMS MERR MUB MOOM RunERR RunUB RunOOM MEMM A B m_exec k_exec m_spec k_spec M_CORRECT K_CORRECT.
+      intros MemM Eff ExtraState MM MRun MPROV MSID MMS MERR MUB MOOM RunERR RunUB RunOOM EQM MLAWS MEMM A B m_exec k_exec m_spec k_spec M_CORRECT K_CORRECT.
 
       unfold exec_correct in *.
       intros ms st VALID.
@@ -2375,7 +2376,7 @@ Module Type MemoryExecMonad (LP : LLVMParams) (MP : MemoryParams LP) (MMSP : Mem
         {X} (x : X),
         exec_correct (ret x) (ret x).
     Proof.
-      intros MemM Eff ExtraState MM MRun MPROV MSID MMS MERR MUB MOOM RunERR RunUB RunOOM H X x.
+      intros MemM Eff ExtraState MM MRun MPROV MSID MMS MERR MUB MOOM RunERR RunUB RunOOM EQM MLAWS H X x.
       cbn; red; cbn.
       intros ms st VALID.
       right; right; right.
@@ -2418,7 +2419,7 @@ Module Type MemoryExecMonad (LP : LLVMParams) (MP : MemoryParams LP) (MMSP : Mem
         (forall a, exec_correct (m_exec a) (m_spec a)) ->
         exec_correct (map_monad_ m_exec xs) (map_monad_ m_spec xs).
     Proof.
-      intros MemM Eff ExtraState MM MRun MPROV MSID MMS MERR MUB MOOM RunERR RunUB RunOOM H A B xs m_exec m_spec H0.
+      intros MemM Eff ExtraState MM MRun MPROV MSID MMS MERR MUB MOOM RunERR RunUB RunOOM EQM MLAWS H A B xs m_exec m_spec H0.
       apply exec_correct_bind.
       eapply exec_correct_map_monad; auto.
       intros a.
@@ -2453,7 +2454,7 @@ Module Type MemoryExecMonad (LP : LLVMParams) (MP : MemoryParams LP) (MMSP : Mem
         {A} (msg : string),
         exec_correct (raise_oom msg) (raise_oom msg : MemPropT MemState A).
     Proof.
-      intros MemM Eff ExtraState MM MRun MPROV MSID MMS MERR MUB MOOM RunERR RunUB RunOOM MemMonad A msg.
+      intros MemM Eff ExtraState MM MRun MPROV MSID MMS MERR MUB MOOM RunERR RunUB RunOOM EQM MLAWS MemMonad A msg.
       cbn.
       red.
       intros ms st VALID.
@@ -2470,7 +2471,7 @@ Module Type MemoryExecMonad (LP : LLVMParams) (MP : MemoryParams LP) (MMSP : Mem
         {A} (msg1 msg2 : string),
         exec_correct (raise_error msg1) (raise_error msg2 : MemPropT MemState A).
     Proof.
-      intros MemM Eff ExtraState MM MRun MPROV MSID MMS MERR MUB MOOM RunERR RunUB RunOOM MemMonad A msg.
+      intros MemM Eff ExtraState MM MRun MPROV MSID MMS MERR MUB MOOM RunERR RunUB RunOOM EQM MLAWS MemMonad A msg.
       cbn.
       red.
       intros ms st VALID.
@@ -2502,7 +2503,7 @@ Module Type MemoryExecMonad (LP : LLVMParams) (MP : MemoryParams LP) (MMSP : Mem
         {A} (m : OOM A),
         exec_correct (lift_OOM m) (lift_OOM m).
     Proof.
-      intros MemM Eff ExtraState MM MRun MPROV MSID MMS MERR MUB MOOM RunERR RunUB RunOOM MemMonad
+      intros MemM Eff ExtraState MM MRun MPROV MSID MMS MERR MUB MOOM RunERR RunUB RunOOM EQM MLAWS MemMonad
              A [NOOM | OOM].
       - apply exec_correct_ret.
       - apply exec_correct_raise_oom.
@@ -2513,7 +2514,7 @@ Module Type MemoryExecMonad (LP : LLVMParams) (MP : MemoryParams LP) (MMSP : Mem
         {A} (m : err A),
         exec_correct (lift_err_RAISE_ERROR m) (lift_err_RAISE_ERROR m).
     Proof.
-      intros MemM Eff ExtraState MM MRun MPROV MSID MMS MERR MUB MOOM RunERR RunUB RunOOM MemMonad
+      intros MemM Eff ExtraState MM MRun MPROV MSID MMS MERR MUB MOOM RunERR RunUB RunOOM EQM MLAWS MemMonad
              A [ERR | NOERR].
       - apply exec_correct_raise_error.
       - apply exec_correct_ret.
@@ -2524,7 +2525,7 @@ Module Type MemoryExecMonad (LP : LLVMParams) (MP : MemoryParams LP) (MMSP : Mem
         {A} (m : ERR A),
         exec_correct (lift_ERR_RAISE_ERROR m) (lift_ERR_RAISE_ERROR m).
     Proof.
-      intros MemM Eff ExtraState MM MRun MPROV MSID MMS MERR MUB MOOM RunERR RunUB RunOOM MemMonad
+      intros MemM Eff ExtraState MM MRun MPROV MSID MMS MERR MUB MOOM RunERR RunUB RunOOM EQM MLAWS MemMonad
              A [[ERR] | NOERR].
       - apply exec_correct_raise_error.
       - apply exec_correct_ret.
@@ -2535,7 +2536,7 @@ Module Type MemoryExecMonad (LP : LLVMParams) (MP : MemoryParams LP) (MMSP : Mem
         len ptr,
         exec_correct (get_consecutive_ptrs ptr len) (get_consecutive_ptrs ptr len).
     Proof.
-      intros MemM Eff ExtraState MM MRun MPROV MSID MMS MERR MUB MOOM RunERR RunUB RunOOM MemMonad
+      intros MemM Eff ExtraState MM MRun MPROV MSID MMS MERR MUB MOOM RunERR RunUB RunOOM EQM MLAWS MemMonad
              len ptr.
       unfold get_consecutive_ptrs.
       eapply exec_correct_bind.
@@ -2550,7 +2551,7 @@ Module Type MemoryExecMonad (LP : LLVMParams) (MP : MemoryParams LP) (MMSP : Mem
         exec_correct fresh_sid fresh_sid.
     Proof.
       red.
-      intros MemM Eff ExtraState MM MRun MPROV MSID MMS MERR MUB MOOM RunERR RunUB RunOOM MemMonad
+      intros MemM Eff ExtraState MM MRun MPROV MSID MMS MERR MUB MOOM RunERR RunUB RunOOM EQM MLAWS MemMonad
              ms st H.
       right.
       eapply MemMonad_run_fresh_sid in H as [st' [sid [EUTT [VALID FRESH]]]].
