src/coq/Handlers/MemoryInterpreters.v
@@ -603,10 +603,10 @@ Module Type MemoryExecInterpreter (LP : LLVMParams) (MP : MemoryParams LP) (MMEP
 
     (* TODO: get rid of this silly hack. *)
     Definition my_handle_memory : MemoryE ~> MemStateFreshT (itree Effout) :=
-      @handle_memory (MemStateFreshT (itree Effout)) _ MemStateFreshT_State _ _ _ _ _ _ _ _ _ _ _ MemStateFreshT_MemMonad.
+      @handle_memory (MemStateFreshT (itree Effout)) _ MemStateFreshT_State _ _ _ _ _ _ _ _ _ _ _ _ _ MemStateFreshT_MemMonad.
 
     Definition my_handle_intrinsic : IntrinsicE ~> MemStateFreshT (itree Effout) :=
-      @handle_intrinsic (MemStateFreshT (itree Effout)) _ MemStateFreshT_State _ _ _ _ _ _ _ _ _ _ _ MemStateFreshT_MemMonad.
+      @handle_intrinsic (MemStateFreshT (itree Effout)) _ MemStateFreshT_State _ _ _ _ _ _ _ _ _ _ _ _ _ MemStateFreshT_MemMonad.
 
     Definition interp_memory_h : Effin ~> MemStateFreshT (itree Effout)
       := case_ E_trigger (case_ my_handle_intrinsic (case_ my_handle_memory F_trigger)).
